lean/src/bpf/spec.lean
@@ -11,38 +11,37 @@ import data.erased
 
 namespace bpf
 
-def trie_safe_with_regs (r : vector value nregs) (p : cfg.trie_program) : Prop :=
-cfg.safe_with_regs p (bpf.reg.of_vector r)
+def trie_safe_with_oracle (o : oracle) (p : cfg.trie_program) : Prop :=
+cfg.safe_with_oracle p o
 
 def trie_safe (p : cfg.trie_program) : Prop :=
 bpf.cfg.safe p
 
 theorem trie_safe_of_erased_regs {p : cfg.trie_program} :
-  (∀ (r : erased (vector value nregs)), trie_safe_with_regs r.out p) →
+  (∀ (o : erased oracle), trie_safe_with_oracle o.out p) →
   trie_safe p :=
 begin
   intros h,
-  simp only [trie_safe, bpf.cfg.safe_iff_safe_with_all_regs],
-  intros r,
-  specialize h (erased.mk (bpf.reg.to_vector r)),
-  simp only [erased.out_mk, trie_safe_with_regs, reg.to_of_vector] at h,
+  intros o,
+  specialize h (erased.mk o),
+  simp only [erased.out_mk, trie_safe_with_oracle] at h,
   exact h
 end
 
-def binary_safe_with_regs (r : vector value nregs) (b : list bool) : Prop :=
+def binary_safe_with_oracle (o : oracle) (b : list bool) : Prop :=
 ∃ (p : cfg.trie_program),
   (decode b).map cfg.trie_program.decode_from_flat = some p ∧
-  cfg.safe_with_regs p (bpf.reg.of_vector r)
+  cfg.safe_with_oracle p o
 
 /-- Top-level specification of BPF program safety.
     A program is safe if and only if there exists a decoded CFG for that program
     and it is safe according to its operational semantics. -/
 @[reducible]
 def binary_safe (b : list bool) : Prop :=
-∀ r, binary_safe_with_regs r b
+∀ o, binary_safe_with_oracle o b
 
 theorem safe_of_erased_regs {b : list bool} :
-  (∀ (r : erased (vector value nregs)), binary_safe_with_regs r.out b) →
+  (∀ (o : erased oracle), binary_safe_with_oracle o.out b) →
   binary_safe b :=
 begin
   intros h r,
